Add processing of sequences for networks.

src/determinism.lean
@@ -4,24 +4,62 @@ namespace determinism
   
   def state := identifier → value  
   def ports := identifier → value 
-  
-  def reaction := (state × ports) → (state × ports)
-  
-  def reaction_determinism (r : reaction) : Prop := ∀ i₁ i₂ : (state × ports), i₁ = i₂ → r i₁ = r i₂
-  theorem reaction_deterministic (r : reaction) : reaction_determinism r :=
-    assume i₁ i₂ : (state × ports),
-    assume h : i₁ = i₂,
-    show r i₁ = r i₂, from congr_arg r h
+  def env := state × ports
 
-  def network := list reaction
-  def send : (state × ports) → network → (state × ports)
-    | i []              := i
-    | i (list.cons r n) := send (r i) n
+  -- REACTION
 
-  def network_determinism (n : network) : Prop := ∀ i₁ i₂ : (state × ports), i₁ = i₂ → send i₁ n = send i₂ n
-  theorem network_deterministic (n : network) : network_determinism n :=
-    assume i₁ i₂ : (state × ports),
-    assume h : i₁ = i₂,
-    show send i₁ n = send i₂ n, from congr (congr_arg send h) (refl n)
+  def reaction := env → env
+  
+  namespace reaction
+
+    def determinism (r : reaction) : Prop := ∀ e₁ e₂ : env, e₁ = e₂ → r e₁ = r e₂
+
+    theorem deterministic (r : reaction) : determinism r :=
+      assume (e₁ e₂ : env) (h : e₁ = e₂),
+      show r e₁ = r e₂, from congr_arg r h
+
+  end reaction
+
+  -- NETWORK
+
+  -- The order produced by a network only describes the *priority* of the reactions, not their connections.
+  inductive network
+    | single (r : reaction) : network
+    | composed (head : reaction) (tail : network) : network
+
+  namespace network
+
+    def process : env → network → env
+      | e (network.single r) := r e
+      | e (network.composed h t) := process (h e) t
+
+    def determinism (n : network) : Prop := ∀ e₁ e₂ : env, e₁ = e₂ → process e₁ n = process e₂ n
+
+    theorem deterministic (n : network) : determinism n :=
+      assume (e₁ e₂ : env) (h : e₁ = e₂),
+      show process e₁ n = process e₂ n, from congr (congr_arg process h) (refl n)
+
+  end network
+
+  -- SEQUENCE NETWORK
+
+  namespace network'
+    
+    -- Given a list of port assignments, an initial state and a network, `process'` ouputs the environment after the networked has
+    -- processed the list of inputs. The `state` output of one reaction is fed as input to the next.
+    def process : (list ports) → state → network → (list env)
+      | [] _ _ := []
+      | (list.cons p t) s n := let e' := (network.process ⟨p, s⟩ n) in list.cons e' (process t e'.1 n) 
+
+    def determinism (n : network) : Prop := 
+      ∀ (p₁ p₂ : list ports) (s₁ s₂ : state), (p₁ = p₂ ∧ s₁ = s₂) → (process p₁ s₁ n) = (process p₂ s₂ n)
+
+    theorem deterministic (n : network) : determinism n :=
+      assume (p₁ p₂ : list ports) (s₁ s₂ : state) (h : p₁ = p₂ ∧ s₁ = s₂),
+      show process p₁ s₁ n = process p₂ s₂ n, from congr (congr (congr_arg process h.left) h.right) (refl n)
+
+  end network'
+
+  
 
 end determinism
